thys/Untyped_Lambda_Calculus/LC_Beta_depth.thy
@@ -7,20 +7,20 @@ begin
 
 (* *)
 
-abbreviation Tsupp :: "nat \<Rightarrow> trm \<Rightarrow> trm \<Rightarrow> var set" where 
-"Tsupp d e1 e2 \<equiv> {} \<union> FFVars_term e1 \<union> FFVars_term e2"
+abbreviation Tsupp :: "nat \<Rightarrow> lterm \<Rightarrow> lterm \<Rightarrow> var set" where 
+"Tsupp d e1 e2 \<equiv> {} \<union> FFVars_Lterm e1 \<union> FFVars_Lterm e2"
 
 lemma fresh: "\<exists>xx. xx \<notin> Tsupp d e1 e2"
-by (metis Lam_avoid term.card_of_FFVars_bounds term.set(2) Un_empty_left)
+by (metis Lam_avoid Lterm.card_of_FFVars_bounds Lterm.set(2) Un_empty_left)
 
-binder_inductive stepD :: "nat \<Rightarrow> trm \<Rightarrow> trm \<Rightarrow> bool" where
+binder_inductive stepD :: "nat \<Rightarrow> lterm \<Rightarrow> lterm \<Rightarrow> bool" where
   Beta: "stepD 0 (App (Lam x e1) e2) (tvsubst (Var(x:=e2)) e1)"
 | AppL: "stepD d e1 e1' \<Longrightarrow> stepD (Suc d) (App e1 e2) (App e1' e2)"
 | AppR: "stepD d e2 e2' \<Longrightarrow> stepD (Suc d) (App e1 e2) (App e1 e2')"
 | Xi: "stepD d e e' \<Longrightarrow> stepD d (Lam x e) (Lam x e')"
   subgoal for R B \<sigma> x1 x2 x3
     by (elim disj_forward exE case_prodE)
-      (auto simp: isPerm_def term.rrename_comps rrename_tvsubst_comp
+      (auto simp: isPerm_def Lterm.rrename_comps rrename_tvsubst_comp
         | ((rule exI[of _ "\<sigma> _"] exI)+, (rule conjI)?, rule refl)
         | ((rule exI[of _ "\<sigma> _"])+; auto))+
   subgoal premises prems for R B x1 x2 x3
