thys/Untyped_Lambda_Calculus/LC_Parallel_Beta.thy
@@ -6,10 +6,10 @@ begin
 
 abbreviation Tsupp where "Tsupp a b \<equiv> FFVars a \<union> FFVars b"
 
-lemma fresh: "\<exists>xx. xx \<notin> Tsupp (t1 :: trm) t2"
-  by (metis (no_types, lifting) exists_var finite_iff_le_card_var term.Un_bound term.set_bd_UNIV)
+lemma fresh: "\<exists>xx. xx \<notin> Tsupp (t1 :: lterm) t2"
+  by (metis (no_types, lifting) exists_var finite_iff_le_card_var Lterm.Un_bound Lterm.set_bd_UNIV)
 
-binder_inductive pstep :: "trm \<Rightarrow> trm \<Rightarrow> bool" where
+binder_inductive pstep :: "lterm \<Rightarrow> lterm \<Rightarrow> bool" where
   Refl: "pstep e e"
 | App: "pstep e1 e1' \<Longrightarrow> pstep e2 e2' \<Longrightarrow> pstep (App e1 e2) (App e1' e2')"
 | Xi: "pstep e e' \<Longrightarrow> pstep (Lam x e) (Lam x e')"
@@ -17,7 +17,7 @@ binder_inductive pstep :: "trm \<Rightarrow> trm \<Rightarrow> bool" where
   subgoal for \<sigma> R B x1 x2
     by (elim disj_forward exE)
       (auto simp: isPerm_def
-         term.rrename_comps rrename_tvsubst_comp
+         Lterm.rrename_comps rrename_tvsubst_comp
          | ((rule exI[of _ "\<sigma> _"] exI)+, (rule conjI)?, rule refl)
          | ((rule exI[of _ "\<sigma> _"])+; auto))+
   subgoal premises prems for R B x1 x2
@@ -32,7 +32,7 @@ binder_inductive pstep :: "trm \<Rightarrow> trm \<Rightarrow> bool" where
       apply hypsubst_thin
       apply (subst (asm) FFVars_tvsubst)
       apply simp
-      apply (unfold term.set)
+      apply (unfold Lterm.set)
       apply (unfold Un_iff de_Morgan_disj)
       apply (erule conjE)+
       apply (subst (2 3) ex_comm)
